attempt to define hoare relation

HoareLc_woc.v
@@ -5,7 +5,7 @@ Require Import Hoare_woc.
 
 
 Definition LContSet := list (label * Assertion).
-Print ceval'.
+
 Definition hoare_triple' (fc : func_context) (P : LContSet) (c : com) (Q : LContSet) : Prop :=
   forall st1 st2 l1 l2 p q,
     In (l1, p) P ->
@@ -14,16 +14,112 @@ Definition hoare_triple' (fc : func_context) (P : LContSet) (c : com) (Q : LCont
     p st1 ->
     q st2.
 
-Definition bridge_between_hoares_re : Prop :=
+Definition func_triple' (fc : func_context) (P : LContSet) (f : func) (Q : LContSet) : Prop :=
+  forall st1 st2 l1 l2 p q,
+    In (l1, p) P ->
+    In (l2, q) Q ->
+    ceval' fc (snd (fc f)) l1 l2 st1 st2 ->
+    p st1 ->
+    q st2.
+
+Inductive matched_label : label -> com -> Prop :=
+  | ML_Skip : matched_label LPure CSkip
+  | ML_Ass : forall X a, matched_label LPure (CAss X a)
+  | ML_Seq : forall l1 l2 c1 c2,
+        matched_label l1 c1 ->
+        matched_label l2 c2 ->
+        matched_label (LSeq l1 l2) (CSeq c1 c2)
+  | ML_If : forall l1 l2 c1 c2 b,
+        matched_label l1 c1 ->
+        matched_label l2 c2 ->
+        matched_label (LIf b l1 l2) (CIf b c1 c2)
+  | ML_While : forall lb c b,
+        matched_label lb c ->
+        matched_label (LWhile b lb) (CWhile b c)
+  | ML_Reentry_here : matched_label LHere CReentry
+  | ML_Reentry_pure : matched_label LPure CReentry.
+
+Definition top (fc : func_context) (f : func) : label :=
+  com_to_label_pure (snd (fc f)).
+
+Definition bottom (fc : func_context) (f : func) : label :=
+  com_to_label_pure (snd (fc f)).
+
+Definition index : Type := (func * label).
+Print sig.
+Print sigT.
+Search sig.
+Definition valid_index (fc : func_context) (lf : list func) (idx : index) : Prop :=
+  In (fst idx) lf /\ matched_label (snd idx) (snd (fc (fst idx))).
+
+Definition index_set (fc : func_context) (lf : list func) : Type :=
+  sig (valid_index fc lf).
+
+Definition param_type (fc : func_context) (lf : list func) : Type :=
+  index_set fc lf -> Type.
+
+Definition invariant (fc : func_context) (lf : list func) (pt : param_type fc lf) : Type := forall i : index_set fc lf, (pt i) -> Assertion.
+
+Definition index_relation (fc : func_context) (lf : list func) (pt : param_type fc lf) : Type := forall i j : index_set fc lf, (pt i) -> (pt j) -> Prop.
+
+Theorem reentry_invariant :
+  forall (fc : func_context) (lf : list func) (f : func) (pt : param_type fc (f :: lf)) (invs : invariant fc (f :: lf) pt) (R : index_relation fc (f :: lf) pt),
+  (forall f',
+  In f' lf ->
+  forall (x : pt (f', top fc f')) (linv : list Assertion),
+    (forall I (j : index_set fc (f' :: nil)),
+      I = (fun st => exists (y : pt j), R (f', top f') j x y /\ (invs j y) st) <-> In I linv) ->
+  func_triple fc lf
+    (((f', top fc f'), (invs (f', top fc f')) x) :: linv) f' (((f', top fc f'), (invs (f', top fc f')) x) :: linv)) ->
+  forall P Q linv,
+  func_triple fc lf
+    (((f, top fc f), P) :: linv) f (((f, top fc f), Q) :: linv).
+
+Theorem bridge_between_hoares_re :
   forall fc lf f' l1 l2 I,
   In f' lf ->
   hoare_triple' fc ((l1, I) :: nil) (snd (fc f')) ((l2, I) :: nil) ->
-  hoare_triple fc I (CReentry lf) I.
-
-Theorem bridge_between_hoares_re_correct : bridge_between_hoares_re.
+  hoare_triple fc lf I CReentry I.
 Proof.
-  unfold bridge_between_hoares_re, hoare_triple', hoare_triple.
+  unfold hoare_triple', hoare_triple.
   intros.
+  apply ceval_multi_ceval' in H1.
 Admitted.
 
-Definition bridge_between_hoares_func : Prop
+Theorem bridge_between_hoares_func :
+  forall fc lf f f' lp lq P Q,
+    In f' lf ->
+    (forall l1 l2 p q,
+      matched_label l1 (snd (fc f')) ->
+      matched_label l2 (snd (fc f')) ->
+      func_triple' fc ((l1, p) :: nil) f' ((l2, q) :: nil)
+        /\ In p lp /\ In q lq) ->
+    (forall p q,
+      In p lp ->
+      In q lq ->
+      q |-- p) ->
+    (exists l1 p,
+    func_triple' fc
+      ((com_to_label_pure (snd (fc f)), P) :: nil)
+      f ((l1, p) :: nil) /\ matched_label l1 (snd (fc f)) /\ In p lp) ->
+    (exists l2 q,
+    func_triple' fc
+      ((l2, q) :: nil) f
+      ((com_to_label_pure (snd (fc f)), Q) :: nil)
+       /\ matched_label l2 (snd (fc f)) /\ In q lq) ->
+    func_triple fc lf P f Q.
+Proof.
+  unfold func_triple', func_triple.
+  intros.
+
+
+
+
+
+
+
+
+
+
+
+
